some roughing out of betree

Splinter/Betree.i.dfy
@@ -2,48 +2,377 @@ include "../lib/Base/total_order.i.dfy"
 include "Tables.i.dfy"
 include "MsgSeq.i.dfy"
 
+/*
+a Betree consists of:
+- Trunk nodes. These have routing information, and link to B+trees that store actual messages.
+  Links include filters that select particular keys, neutralize old messages.
+- Immutable B+trees, allocated in big (many-MB?) chunks, store a batch of messages from
+  a rectangle of some keyrange * sequence number window.
+- Flush is two steps:
+  - "Pushdown"? logically pushes a sub-rectangle of messages to a child trunk node, done by
+    forwarding the references.
+  - Compact rewrites content from input B+trees to an output B+tree, pushing the input trees
+    closer to being freed. This is garbage collection.
+- Lookup must:
+  - follow an appropriate trunk path
+  - Collect non-excluded messages from every linked B+tree
+- Allocation must account for:
+  - Used trunk nodes. (One CU allocated in an entire AU, evidently.)
+  - Batches of CUs (AUs) used to build a B+tree.
+
+So Betree.lookup is a series of trunk nodes, their CUs,
+  plus for each a B+tree.lookup, which itself is a series of CUs.
+
+  So maybe the thing to do is stub out the B+tree interface that this thing is going to
+  take as a submodule.
+
+  Also, how are we going to do:
+  * dependency tracking for when we can free B+trees
+    * how do we write down that change in allocation?
+    * at this layer, maybe define the Betree allocation as the union of the reachable B+tree
+      allocations?
+  * indirection table?  each time we replace a trunk node, we want to
+    - allocate a new CU to store it in
+    - link the parent to this new CU
+    - This process doesn't need reference counting, but it does affect the reference
+      counts for the B+trees. WAIT YES IT DOES it's a Bedag -- for clone.
+    - We do need to adjust allocations when we make the swap.
+
+  How to B+trees get incrementally constructed?
+    - At this layer in the refinement stack, maybe they just get incrementally allocated,
+    in a way that the increments never get frozen?
+
+  Allocation strategy.
+  * At this refinement layer, we'll identify the
+    - reachable trunk CUs (Identified by lookups? gulp) and
+    - reachable B+tree CU sets.
+    - and then our sb.alloc will reflect those sets whenever we freeze.
+
+  * In next layer down, we can't require faulting the entire tree in to compute the alloc,
+    so we'll attach it to invariants that track:
+    - an allocation table read from the disk representing the base (persistent) image
+    - When we de/allocate a trunk CU or B+tree set<CU>, we'll subtract/add them to the table
+  Will the invariant connection be via a recursive definition? Gulp. Definitely not if
+    trunks form a DAG.
+  Will the invariant connection simply be induction invariants that
+    - every reachable thing is in the set
+    - everything in the set is reachable (ew)
+    - no reachable thing overlaps with another reachable thing (ew ew)
+  Maybe
+    - we ghostily know the set of reachable B+trees. (Can we marshal ghost data across a restart?)
+    - we ghostily know the set of reachable trunks.
+    - we maintain an invariant between the set of IReads sets of those data structures
+    that gives mutual disjointness and that they union to the allocation set.
+
+  Indirection table:
+  - There are two kinds of things that need refcounting: B+trees and trunks.
+  - We used to think we'd reference count allocated CUs. That doesn't make any sense.
+  - But how do we *name* the B+trees and name the trunks? By their roots? Why not? CUs are
+    disjoint, so root CUs are unique... and that's also how they're named in pointers.
+
+  - How many trunks are there? How many B+trees?
+    - I think we're going to end up storing a table in memory that's shaped very much
+    like an allocation table, but has counters.
+    - It's going to count refs to CUs.
+      - Can we represent this one relationally against a whole DiskView? I think we can!
+      forall reachable trunks forall b+trees count once?
+    - And then another table is going to connect CU roots to all the CUs (or rather all the AUs)
+      for a given data structure.
+      - in particular, this second table, at this layer, can be represented by just reading the
+      underlying data structures!
+
+*/
+
+module MapExtra {
+  import opened Sequences
+  import opened Maps
+
+  // TODO move to library
+  // Collapse a sequence of maps with Map
+}
+
 module BetreeMachineMod {
   import opened Options
+  import opened Sequences
+  import opened Maps
+  import opened MapExtra
   import opened MessageMod
   import opened InterpMod
   import opened AllocationMod
   import opened MsgSeqMod
-  import opened IndirectionTableMod
+  import IndirectionTableMod
   import CacheIfc
 
   datatype Superblock = Superblock(
     itbl: IndirectionTableMod.Superblock,
-    rootIdx: IndirectionTableMod.IndirectionTable,
-    seqEnd: nat)
+    endSeq: LSN)
 
-  datatype Variables = Variables()
+  datatype Frozen = Idle | Frozen(
+    indTbl: IndirectionTableMod.IndirectionTable,
+    endSeq: LSN)
 
-  predicate Query(v: Variables, v': Variables, key: Key, value: Value)
+  datatype Variables = Variables(
+    indTbl: IndirectionTableMod.IndirectionTable,
+    memBuffer: map<Key, Message>,  // Real Splinter (next layer down? :v) has >1 memBuffers so we can be inserting at the front while flushing at the back.
+    // TODO add a membuffer to record LSN; a frozen-like transition to keep one membuffer available
+    // for filling while packing the other into a b+tree in the top trunk.
+    // OR just have freeze drain the membuffer, introducing a write hiccup every 20GB.
+    nextSeq: LSN,  // exclusive
+    frozen: Frozen
+  )
+
+  type TrunkId = nat
+  function RootId() : TrunkId { 0 }
+
+  datatype TrunkNode = TrunkNode()
+  function parseTrunkNode(b: UninterpretedDiskPage) : Option<TrunkNode>
+    // TODO
+  function marshalTrunkNode(node: TrunkNode) : UninterpretedDiskPage
+    // TODO
+
+  datatype NodeAssignment = NodeAssignment(id: TrunkId, cu: CU, node: TrunkNode)
   {
-    && true //TODO
+    predicate InIndTable(v: Variables) {
+      && id in v.indTbl
+      && v.indTbl[id] == cu
+    }
+    predicate Valid(v: Variables, cache: CacheIfc.Variables) {
+      && InIndTable(v)
+      && var unparsedPage := CacheIfc.ReadValue(cache, cu);
+      && unparsedPage.Some?
+      && Some(node) == parseTrunkNode(unparsedPage.value)
+    }
+  }
+
+  // TODO find in library
+  function CombineMessages(newer: Message, older: Message) : Message
+  function EvaluateMessage(m: Message) : Value
+
+  function MessageFolder(newer: map<Key,Message>, older: map<Key,Message>) : map<Key,Message>
+  {
+		map x : Key | (x in newer.Keys + older.Keys) ::
+      if x in newer
+      then if x in older
+        then CombineMessages(newer[x], older[x])
+        else newer[x]
+      else older[x]
+  }
+
+  datatype TrunkStep = TrunkStep(
+    na: NodeAssignment,
+    msgs: map<Key, Message>
+    // , branchMsgs: seq<map<Key, Message>>, branchAssigment: BranchAssignment   ...
+    )
+  datatype TrunkPath = TrunkPath(k: Key, steps: seq<TrunkStep>)
+  {
+    predicate ValidPrefix(cache: CacheIfc.Variables) {
+      true // some path from the root
+    }
+
+    predicate Valid(cache: CacheIfc.Variables) {
+      && ValidPrefix(cache)
+      && true // no nodes below this one for k.
+    }
+
+    function Decode() : Value
+    {
+      // filter Messages on k, I guess
+      var unflattenedMsgs := seq(|steps|, i requires 0<=i<|steps| => steps[i].msgs);
+      var flattenedMsgs := FoldLeft(MessageFolder, map[], unflattenedMsgs);
+      if k in flattenedMsgs then EvaluateMessage(flattenedMsgs[k]) else DefaultValue()
+    }
+  }
+
+  predicate Query(v: Variables, v': Variables, cache: CacheIfc.Variables, key: Key, value: Value, trunkPath: TrunkPath)
+  {
+    && trunkPath.Valid(cache)
+    && trunkPath.k == key
+    && trunkPath.Decode() == value
     && v' == v
   }
+
+  function MakeValueMessage(value:Value) : Message
+    // TODO somewhere somehow
 
   predicate Put(v: Variables, v': Variables, key: Key, value: Value)
   {
-    && true //TODO
-    && v' == v
+    && var newMessage := MakeValueMessage(value);
+    && v' == v.(memBuffer := v.memBuffer[key := newMessage], nextSeq := v.nextSeq + 1)
   }
 
-  predicate Internal(v: Variables, v': Variables)
+  datatype FlushRec = FlushRec(
+    trunkPath: TrunkPath,
+    newParent: NodeAssignment,
+    newChild: NodeAssignment)
   {
-    false
+    predicate WF() {
+      2<=|trunkPath.steps|
+    }
+    predicate Valid(cache: CacheIfc.Variables) {
+      && WF()
+      && trunkPath.ValidPrefix(cache)
+    }
+    function ParentStep() : TrunkStep
+      requires WF()
+      { trunkPath.steps[|trunkPath.steps|-2] }
+    function ChildStep() : TrunkStep
+      requires WF()
+      { trunkPath.steps[|trunkPath.steps|-1] }
+    function ParentNode() : TrunkNode
+      requires WF()
+      { ParentStep().na.node }
+    function ChildNode() : TrunkNode
+      requires WF()
+      { ChildStep().na.node }
+  }
+
+  predicate FlushesNodes(oldParent: TrunkNode, oldChild: TrunkNode, newParent: TrunkNode, newChild: TrunkNode) {
+    true // TODO
+  }
+  
+  predicate CUIsAllocatable(cu: CU)
+  {
+    && true // TODO cu unallocated across all live views
+  }
+
+  // Internal operation; noop
+  predicate Flush(v: Variables, v': Variables, cache: CacheIfc.Variables, cacheOps: CacheIfc.Ops, flush: FlushRec)
+  {
+    && flush.Valid(cache)
+    // TODO keep the parent's trunkId, but move the child, so that other nodes' outbound links
+    // to existing child don't change.
+    && FlushesNodes(flush.ParentNode(), flush.ChildNode(), flush.newParent.node, flush.newChild.node)
+    && flush.newParent.id == flush.ParentStep().na.id  // parent keeps its id
+    && true // UnusedId(flush.newChild.id) child gets id unallocated in eph ind tbl
+    && CUIsAllocatable(flush.newParent.cu)
+    && CUIsAllocatable(flush.newChild.cu)
+    && cacheOps == [
+      CacheIfc.Write(flush.newParent.cu, marshalTrunkNode(flush.newParent.node)),
+      CacheIfc.Write(flush.newChild.cu, marshalTrunkNode(flush.newChild.node))
+      ]
+    && v' == v.(indTbl := v.indTbl
+      [flush.ParentStep().na.id := flush.newParent.cu]
+      [flush.newChild.id := flush.newChild.cu])  // TODO breaks other dag neighbors
+  }
+
+  predicate MergeBuffer(oldNode: TrunkNode, memBuffer: map<Key, Message>, newNode: TrunkNode)
+  {
+    true // tODO
+  }
+
+  // Internal
+  // drain mem buffer into a B+tree in the root trunk node
+  predicate DrainMemBuffer(v: Variables, v': Variables, cache: CacheIfc.Variables, cacheOps: CacheIfc.Ops, oldRoot: NodeAssignment, newRoot: NodeAssignment)
+  {
+    && oldRoot.id == RootId()
+    && oldRoot.Valid(v, cache)
+    && newRoot.id == RootId()
+    // when we're done, newRoot.Valid(v', cache')
+
+    && CUIsAllocatable(newRoot.cu)
+    && MergeBuffer(oldRoot.node, v.memBuffer, newRoot.node)
+    && cacheOps == [ CacheIfc.Write(newRoot.cu, marshalTrunkNode(newRoot.node)) ]
+    && v' == v.(
+      indTbl := v.indTbl[RootId() := newRoot.cu],
+      memBuffer := map[]
+      )
+  }
+
+  datatype CompactReceipt = CompactReceipt(path: TrunkPath, newna: NodeAssignment)
+  {
+    predicate WF() {
+      && 0 < |path.steps|
+    }
+    function Oldna() : NodeAssignment
+      requires WF()
+    {
+      Last(path.steps).na
+    }
+    predicate Valid(cache: CacheIfc.Variables)
+    {
+      && WF()
+      && path.Valid(cache)
+      && Oldna().id == newna.id
+    }
+  }
+
+  predicate EquivalentNodes(a: TrunkNode, b: TrunkNode) {
+    true // TODO
+  }
+
+  // Internal operation; noop
+  // Rearrange mem buffers in some node
+  predicate CompactBranch(v: Variables, v': Variables, cache: CacheIfc.Variables, cacheOps: CacheIfc.Ops, r: CompactReceipt)
+  {
+    && r.Valid(cache)
+    && CUIsAllocatable(r.newna.cu)
+    && EquivalentNodes(r.Oldna().node, r.newna.node)  // Buffer replacements
+      // TODO need to establish replacement B+tree is correct
+    && cacheOps == [ CacheIfc.Write(r.newna.cu, marshalTrunkNode(r.newna.node)) ]
+    && v' == v.(indTbl := v.indTbl[r.newna.id := r.newna.cu])
+  }
+
+  predicate Freeze(v: Variables, v': Variables)
+  {
+    && v.frozen.Idle?
+    && v.memBuffer == map[]  // someday we'd like to avoid clogging the memtable during freeze, but...
+    && v' == v.(frozen := Frozen(v.indTbl,  v.nextSeq))
+  }
+
+  predicate KnowFrozenIsClean(v: Variables, sb: Superblock, cache: CacheIfc.Variables)
+  {
+    true // TODO
   }
 
   predicate CommitStart(v: Variables, v': Variables, cache: CacheIfc.Variables, sb: Superblock, newBoundaryLSN: LSN)
   {
-    && true //TODO
+    && v.frozen.Frozen?
+    && KnowFrozenIsClean(v, sb, cache)
+    && sb.endSeq == v.frozen.endSeq
+    && v' == v
   }
 
-  predicate CommitComplete(s: Variables, s': Variables, cache: CacheIfc.Variables, sb: Superblock)
+  predicate CommitComplete(v: Variables, v': Variables, cache: CacheIfc.Variables, sb: Superblock)
   {
-    && true //TODO
+    // TODO need to update the persistent table to keep our allocation set correct
+    && v' == v.(frozen := Idle)
   }
+
+/*
+  predicate ReachableTrunk(sb: Superblock, trunkRoot: CU)
+  {
+    && true // TODO -- lookup-y definition
+  }
+
+  predicate ReachableBranch(cache: CacheIfc.Variables, sb: Superblock, branchRoot: CU)
+  {
+    // NB: no indirection from trunks to branches -- but there is refcounting here. Use multiset representation for IReads, I guess.
+    exists trunkCU, trunkNode, branchIdx ::
+      && ReachableTrunk(sb, trunkCU)
+      && var unparsedPage := CacheIfc.ReadValue(cache, trunkCU);
+      && unparsedPage.Some?
+      && var trunkNode := parseTrunkNode(unparsedPage.value);
+      && trunkNode.Some?
+      // TODO trunk nodes need some guts
+      //&& trunkNode.value.branches[branchIdx] == branchRoot
+  }
+
+  predicate BranchMember(sb: Superblock, branchRoot: CU, block: CU)
+  {
+    && true // TODO -- this defn belongs inside branch module
+  }
+
+  predicate ReachableBlock(cache: CacheIfc.Variables, sb: Superblock, cu: CU)
+  {
+    || ReachableTrunk(cache, trunkCu)
+    || (exists branch ::
+      && ReachableBranch(cache, sb, trunkCu)
+      && BranchMember(branchRoot, cu))
+  }
+*/
+
+  // And then IReads <= ReachableBlocks == alloc.
+  // We can prove this because anything in IReads justifies ReachableTrunk (and maybe BranchMember).
 }
 
 module BetreeInterpMod {
@@ -84,7 +413,7 @@ module BetreeInterpMod {
   function IM(dv: DiskView, sb: Superblock) : (i:Interp)
     ensures i.WF()
   {
-    Interp(imap key | key in AllKeys() :: IMKey(dv, sb, key), sb.seqEnd)
+    Interp(imap key | key in AllKeys() :: IMKey(dv, sb, key), sb.endSeq)
   }
 
   function IReadsKey(dv: DiskView, itbl: Option<IndirectionTableMod.IndirectionTable>, key: Key) : set<AU> {
